redefining groups, fixing the pike tree invariant preservation proof

Regex.v
@@ -1,82 +1,10 @@
 Require Import List Lia.
 Import ListNotations.
 
-(** * Characters and Strings  *)
-Parameter Char:Type.
-Definition string := list Char.
+Require Import Chars.
+Require Import Groups.
 
-(* In the semantics, the input string is represented with both the next characters to read
-   and the reversed list of previously read characters (in case we change direction for a lookbehind) *)
-Inductive input : Type :=
-| Input (next: string) (pref: string).
-
-Parameter char_eq_dec : forall (x y : Char), { x = y } + { x <> y }.
-Definition string_eq_dec : forall (x y : string), { x = y } + { x <> y }.
-Proof.
-  decide equality. apply char_eq_dec.
-Defined.
-Definition input_eq_dec: forall (i1 i2: input), { i1 = i2 } + { i1 <> i2 }.
-Proof. decide equality; apply string_eq_dec. Defined.
-
-(* indicating which character is a word character for anchors *)
-Parameter word_char : Char -> bool.
-
-(** * Character Descriptors  *)
-(* by character descriptors, we mean everything that can represent a single character *)
-(* the character itself, the dot, an escape, a character group like \d, character classes *)
-Parameter char_descr : Type.
-
-(* common character descriptors *)
-Parameter dot : char_descr.
-(* dot is not all characters without multiline flag *)
-Parameter all: char_descr.
-(* single char *)
-Parameter single : Char -> char_descr.
-
-Parameter char_match : Char -> char_descr -> bool.
-
-Axiom single_match:
-  forall c1 c2, char_match c1 (single c2) = true <-> c1 = c2.
-
-Axiom all_match:
-  forall c, char_match c all = true.
-
-Parameter char_descr_eq_dec : forall (cd1 cd2: char_descr), { cd1 = cd2 } + { cd1 <> cd2 }.
-
-
-(** * Reading Characters in the String *)
-
-(* read_char cd i returns None if the next character of i is accepted by cd *)
-(* otherwise it returns the next input after reading the character, as well as the character actually read *)
-Definition read_char (cd:char_descr) (i:input) : option (Char * input) :=
-  match i with
-  | Input next pref =>
-      match next with
-      | [] => None
-      | h::next' => if char_match h cd
-                  then Some (h, Input next' (h::pref))
-                  else None
-      end
-  end.
-
-
-Definition next_str (i:input) : string :=
-  match i with
-  | Input s _ => s
-  end.
-
-Definition current_str (i:input) : string :=
-  match i with
-  | Input next pref => next
-  end.
-
-Definition init_input (str:string) : input :=
-  Input str [].
-
- 
 (** * Regex Syntax  *)
-Definition group_id : Type := nat.
-
 Inductive regex : Type :=
 | Epsilon 
 | Character (cd : char_descr)   (* includes character classes and dot *)
@@ -100,37 +28,4 @@ Fixpoint def_groups (r:regex) : list group_id :=
   | Star r1 => def_groups r1
   | Group id r1 => id::(def_groups r1)  
   end.
-
-(* Storing the values of each group and a function indicating if each group is opened or closed *)
-Definition group_map : Type :=
-  (group_id -> option string) * (group_id -> bool).
-
-Definition empty_group_map : group_map :=
-  (fun _ => None, fun _ => false).
-
-Definition open_group (g:group_map) (id:group_id) : group_map :=
-  ((fun id2 => if (Nat.eqb id2 id) then Some [] else fst g id2),
-    (fun id2 => if (Nat.eqb id2 id) then true else snd g id2)).
-
-Definition close_group (g:group_map) (id:group_id) : group_map :=
-  ((fst g),
-    (fun id2 => if (Nat.eqb id2 id) then false else (snd g) id2)).
-
-Definition add_char (g:group_map) (c:Char) : group_map :=
-  ((fun id =>
-      if snd g id then
-        match fst g id with
-        | None => Some [c]       (* None should never happen when the boolean is true *)
-        | Some l  => Some (c::l)
-        end
-      else fst g id),
-    snd g).
-
-Definition reset_group (g:group_map) (id:group_id) : group_map :=
-  ((fun id2 => if (Nat.eqb id2 id) then None else fst g id2),
-    (* we could let snd g unchanged: when we reset, the groups should be closed *)
-    (fun id2 => if (Nat.eqb id2 id) then false else snd g id2)).
-
-Definition reset_groups (g:group_map) (idl:list group_id) : group_map :=
-  List.fold_left reset_group idl g.
 
