Chars.v
@@ -1,0 +1,74 @@
+Require Import List Lia.
+Import ListNotations.
+
+(** * Characters and Strings  *)
+Parameter Char:Type.
+Definition string := list Char.
+
+(* In the semantics, the input string is represented with both the next characters to read
+   and the reversed list of previously read characters (in case we change direction for a lookbehind) *)
+Inductive input : Type :=
+| Input (next: string) (pref: string).
+
+Parameter char_eq_dec : forall (x y : Char), { x = y } + { x <> y }.
+Definition string_eq_dec : forall (x y : string), { x = y } + { x <> y }.
+Proof.
+  decide equality. apply char_eq_dec.
+Defined.
+Definition input_eq_dec: forall (i1 i2: input), { i1 = i2 } + { i1 <> i2 }.
+Proof. decide equality; apply string_eq_dec. Defined.
+
+(* indicating which character is a word character for anchors *)
+Parameter word_char : Char -> bool.
+
+(** * Character Descriptors  *)
+(* by character descriptors, we mean everything that can represent a single character *)
+(* the character itself, the dot, an escape, a character group like \d, character classes *)
+Parameter char_descr : Type.
+
+(* common character descriptors *)
+Parameter dot : char_descr.
+(* dot is not all characters without multiline flag *)
+Parameter all: char_descr.
+(* single char *)
+Parameter single : Char -> char_descr.
+
+Parameter char_match : Char -> char_descr -> bool.
+
+Axiom single_match:
+  forall c1 c2, char_match c1 (single c2) = true <-> c1 = c2.
+
+Axiom all_match:
+  forall c, char_match c all = true.
+
+Parameter char_descr_eq_dec : forall (cd1 cd2: char_descr), { cd1 = cd2 } + { cd1 <> cd2 }.
+
+
+(** * Reading Characters in the String *)
+
+(* read_char cd i returns None if the next character of i is accepted by cd *)
+(* otherwise it returns the next input after reading the character, as well as the character actually read *)
+Definition read_char (cd:char_descr) (i:input) : option (Char * input) :=
+  match i with
+  | Input next pref =>
+      match next with
+      | [] => None
+      | h::next' => if char_match h cd
+                  then Some (h, Input next' (h::pref))
+                  else None
+      end
+  end.
+
+
+Definition next_str (i:input) : string :=
+  match i with
+  | Input s _ => s
+  end.
+
+Definition current_str (i:input) : string :=
+  match i with
+  | Input next pref => next
+  end.
+
+Definition init_input (str:string) : input :=
+  Input str [].
