Groups.v
@@ -1,0 +1,51 @@
+(* Defining Capture Groups Registers *)
+(* Keeping an index of when was a group opened and closed *)
+
+Require Import List Lia.
+Import ListNotations.
+
+
+Require Import Chars.
+
+Definition group_id : Type := nat.
+
+(* Storing the values of each group and a function indicating if each group is opened or closed *)
+Parameter group_map: Type.
+Parameter empty_group_map : group_map.
+
+Parameter open_group: group_map -> group_id -> nat -> group_map.
+Parameter close_group: group_map -> group_id -> nat -> group_map.
+Parameter reset_group: group_map -> group_id -> group_map.
+
+Definition reset_groups (g:group_map) (idl:list group_id) : group_map :=
+  List.fold_left reset_group idl g.
+
+Parameter get_begin : group_map -> group_id -> option nat.
+Parameter get_end : group_map -> group_id -> option nat.
+
+
+(** * Axiomatisation  *)
+
+Axiom empty_none_begin:
+  forall gid, get_begin empty_group_map gid = None.
+
+Axiom empty_none_end:
+  forall gid, get_end empty_group_map gid = None.
+
+Axiom group_open_begin:
+  forall gid idx gm, get_begin (open_group gm gid idx) gid = Some idx.
+
+Axiom group_close_end:
+  forall gid idx gm, get_end (close_group gm gid idx) gid = Some idx.
+
+Axiom get_reset_begin:
+  forall gid gm, get_begin (reset_group gm gid) gid = None.
+
+Axiom get_reset_end:
+  forall gid gm, get_end (reset_group gm gid) gid = None.
+
+Axiom get_other_begin_open:
+  forall gid1 gid2 gm idx,
+    gid1 <> gid2 ->
+    get_begin (open_group gm gid1 idx) gid2 = get_begin gm gid2.
+(* TODO: and so many more like this *)
